WIP: sim, match genv

imp/Imp.v
@@ -280,9 +280,9 @@ Record program : Type := mk_program {
     let ifs := List.map (fun p => fst p) prog_funs in
     ["malloc"; "free"] ++ evs ++ efs ++ ivs ++ ifs;
   defs : list (gname * Sk.gdef) :=
-    let vs := (List.map (fun '(vn, vv) => (vn, Sk.Gvar vv)) prog_vars) in
     let fs := (List.map (fun '(fn, _) => (fn, Sk.Gfun)) prog_funs) in
-    vs ++ fs;
+    let vs := (List.map (fun '(vn, vv) => (vn, Sk.Gvar vv)) prog_vars) in
+    fs ++ vs;
 }.
 
 Definition lift (p : program) : programL :=
